Did a bunch of work on type checking

02Typed/Typechecking.thy
@@ -2,20 +2,352 @@ theory Typechecking
   imports Typed "../01Source/Named" "../00Utils/Unification/Unification"
 begin
 
+datatype hexpr = 
+  HVar var
+  | HConst nat
+  | HLam var uexpr hexpr
+  | HApp hexpr hexpr
+
+primrec hsubst :: "subst \<Rightarrow> hexpr \<Rightarrow> hexpr" where
+  "hsubst sub (HVar x) = HVar x"
+| "hsubst sub (HConst k) = HConst k"
+| "hsubst sub (HLam x t e) = HLam x (subst sub t) (hsubst sub e)"
+| "hsubst sub (HApp e\<^sub>1 e\<^sub>2) = HApp (hsubst sub e\<^sub>1) (hsubst sub e\<^sub>2)"
+
 primrec erase :: "texpr \<Rightarrow> nexpr" where
   "erase (TVar x) = NVar x"
 | "erase (TConst k) = NConst k"
 | "erase (TLam x t e) = NLam x (erase e)"
 | "erase (TApp e\<^sub>1 e\<^sub>2) = NApp (erase e\<^sub>1) (erase e\<^sub>2)"
 
-primrec typecheck :: "nexpr \<rightharpoonup> texpr \<times> ty" where
-  "typecheck (NVar x) = undefined"
+primrec typecheck' :: "subst \<Rightarrow> var set \<Rightarrow> nexpr \<rightharpoonup> 
+    hexpr \<times> uexpr \<times> var set \<times> (var \<rightharpoonup> uexpr)" where
+  "typecheck' \<Gamma> vs (NVar x) = (case \<Gamma> x of 
+      Some t \<Rightarrow> Some (HVar x, t, vs, \<Gamma>) 
+    | None \<Rightarrow> None)"
+| "typecheck' \<Gamma> vs (NConst k) = Some (HConst k, Ctor ''Base'' [], vs, \<Gamma>)"
+| "typecheck' \<Gamma> vs (NLam x e) = (
+    let v = fresh vs
+    in case typecheck' (\<Gamma>(x \<mapsto> Var v)) (insert v vs) e of
+        Some (e', t, vs', \<Gamma>') \<Rightarrow> (case \<Gamma>' x of 
+          Some t' \<Rightarrow> Some (HLam x t' e', Ctor ''Arrow'' [t', t], vs', (\<Gamma>'(x := \<Gamma> x)))
+        | None \<Rightarrow> None)
+      | None \<Rightarrow> None)"
+| "typecheck' \<Gamma> vs (NApp e\<^sub>1 e\<^sub>2) = (case typecheck' \<Gamma> vs e\<^sub>1 of
+      Some (e\<^sub>1', Ctor k [t\<^sub>1, t\<^sub>2], vs', \<Gamma>') \<Rightarrow> (
+        if k = ''Arrow'' then case typecheck' \<Gamma>' vs' e\<^sub>2 of
+            Some (e\<^sub>2', t\<^sub>3, vs'', \<Gamma>'') \<Rightarrow> (case unify t\<^sub>1 t\<^sub>2 of     
+              Some sub \<Rightarrow> Some (HApp (hsubst sub e\<^sub>1') (hsubst sub e\<^sub>2'), subst sub t\<^sub>2, vs'', 
+                                map_option (subst sub) \<circ> \<Gamma>'')
+            | None \<Rightarrow> None)
+          | None \<Rightarrow> None
+        else None)
+    | _ \<Rightarrow> None)"
+
+fun typeify :: "uexpr \<Rightarrow> ty" where
+  "typeify (Var v) = TyVar v"
+| "typeify (Ctor k []) = (if k = ''Base'' then Base else undefined)"
+| "typeify (Ctor k [t\<^sub>1, t\<^sub>2]) = 
+    (if k = ''Arrow'' then Arrow (typeify t\<^sub>1) (typeify t\<^sub>2) else undefined)"
+| "typeify (Ctor k ts) = undefined"
+
+fun valid_ty_uexpr :: "uexpr \<Rightarrow> bool" where
+  "valid_ty_uexpr (Var v) = True"
+| "valid_ty_uexpr (Ctor k []) = (k = ''Base'')"
+| "valid_ty_uexpr (Ctor k [t\<^sub>1, t\<^sub>2]) = (k = ''Arrow'' \<and> valid_ty_uexpr t\<^sub>1 \<and> valid_ty_uexpr t\<^sub>2)"
+| "valid_ty_uexpr (Ctor k ts) = False"
+
+definition valid_ty_subst :: "subst \<Rightarrow> bool" where
+  "valid_ty_subst \<Gamma> = (\<forall>t \<in> ran \<Gamma>. valid_ty_uexpr t)"
+
+primrec solidify :: "hexpr \<Rightarrow> texpr" where
+  "solidify (HVar x) = TVar x"
+| "solidify (HConst k) = TConst k"
+| "solidify (HLam x t e) = TLam x (typeify t) (solidify e)"
+| "solidify (HApp e\<^sub>1 e\<^sub>2) = TApp (solidify e\<^sub>1) (solidify e\<^sub>2)"
+
+primrec valid_ty_hexpr :: "hexpr \<Rightarrow> bool" where
+  "valid_ty_hexpr (HVar x) = True"
+| "valid_ty_hexpr (HConst k) = True"
+| "valid_ty_hexpr (HLam x t e) = (valid_ty_uexpr t \<and> valid_ty_hexpr e)"
+| "valid_ty_hexpr (HApp e\<^sub>1 e\<^sub>2) = (valid_ty_hexpr e\<^sub>1 \<and> valid_ty_hexpr e\<^sub>2)"
+
+fun typecheck :: "nexpr \<rightharpoonup> texpr \<times> ty" where
+  "typecheck e = (case typecheck' Map.empty {} e of
+      Some (e', t, vs, \<Gamma>) \<Rightarrow> Some (solidify e', typeify t)
+    | None \<Rightarrow> None)"
+
+fun tsubsts :: "subst \<Rightarrow> ty \<Rightarrow> ty" where
+  "tsubsts sub (TyVar y) = (case sub y of Some t \<Rightarrow> typeify t | None \<Rightarrow> TyVar y)"
+| "tsubsts sub Base = Base"
+| "tsubsts sub (Arrow t\<^sub>1 t\<^sub>2) = Arrow (tsubsts sub t\<^sub>1) (tsubsts sub t\<^sub>2)"
+
+primrec tsubstt :: "subst \<Rightarrow> texpr \<Rightarrow> texpr" where
+  "tsubstt sub (TVar x) = TVar x"
+| "tsubstt sub (TConst k) = TConst k"
+| "tsubstt sub (TLam x t e) = TLam x (tsubsts sub t) (tsubstt sub e)"
+| "tsubstt sub (TApp e\<^sub>1 e\<^sub>2) = TApp (tsubstt sub e\<^sub>1) (tsubstt sub e\<^sub>2)"
+
+lemma [simp]: "valid_ty_uexpr t \<Longrightarrow> typeify (subst sub t) = tsubsts sub (typeify t)"
+  by (induction t rule: typeify.induct) (simp_all split: option.splits)
+
+lemma [simp]: "valid_ty_subst Map.empty"
+  by (simp add: valid_ty_subst_def)
+
+lemma [simp]: "valid_ty_subst \<Gamma> \<Longrightarrow> 
+    map_option (typeify \<circ> subst sub) (\<Gamma> x) = map_option (tsubsts sub \<circ> typeify) (\<Gamma> x)"
+  by (cases "\<Gamma> x") (auto simp add: valid_ty_subst_def ran_def)
+
+lemma [simp]: "valid_ty_subst \<Gamma> \<Longrightarrow> 
+    map_option (typeify \<circ> subst sub) \<circ> \<Gamma> = map_option (tsubsts sub \<circ> typeify) \<circ> \<Gamma>"
+  by auto
+
+lemma [simp]: "valid_ty_hexpr e \<Longrightarrow> solidify (hsubst sub e) = tsubstt sub (solidify e)"
+  by (induction e) simp_all
+
+lemma [simp]: "erase (tsubstt sub e) = erase e"
+  by (induction e) simp_all
+
+lemma [simp]: "valid_ty_subst \<Gamma> \<Longrightarrow> valid_ty_uexpr t \<Longrightarrow> valid_ty_subst (\<Gamma>(x \<mapsto> t))"
+  by (auto simp add: valid_ty_subst_def ran_def)
+
+lemma [simp]: "valid_ty_subst \<Gamma> \<Longrightarrow> valid_ty_subst \<Gamma>' \<Longrightarrow> valid_ty_subst (\<Gamma>(x := \<Gamma>' y))"
+  by (auto simp add: valid_ty_subst_def ran_def)
+
+lemma [simp]: "valid_ty_uexpr t \<Longrightarrow> valid_ty_subst sub \<Longrightarrow> valid_ty_uexpr (subst sub t)"
+  by (induction t rule: valid_ty_uexpr.induct) 
+     (auto simp add: valid_ty_subst_def ran_def split: option.splits)
+
+lemma [simp]: "valid_ty_subst \<Gamma> \<Longrightarrow> valid_ty_subst sub \<Longrightarrow> 
+    valid_ty_subst (map_option (subst sub) \<circ> \<Gamma>)"
+  by (auto simp add: valid_ty_subst_def ran_def)
+
+lemma [elim]: "valid_ty_subst \<Gamma> \<Longrightarrow> \<Gamma> x = Some t \<Longrightarrow> valid_ty_uexpr t"
+  by (auto simp add: valid_ty_subst_def ran_def)
+
+lemma [elim]: "valid_ty_uexpr t\<^sub>1 \<Longrightarrow> valid_ty_uexpr t\<^sub>2 \<Longrightarrow> unify t\<^sub>1 t\<^sub>2 = Some sub \<Longrightarrow> 
+    valid_ty_subst sub"                                  
+  by (auto simp add: valid_ty_subst_def)
+
+lemma [simp]: "valid_ty_subst sub \<Longrightarrow> valid_ty_hexpr e \<Longrightarrow> valid_ty_hexpr (hsubst sub e)"
+  by (induction e) simp_all
+
+lemma tc_tsubstt [simp]: "\<Gamma> \<turnstile>\<^sub>n e : t \<Longrightarrow> 
+  map_option (tsubsts sub) \<circ> \<Gamma> \<turnstile>\<^sub>n tsubstt sub e : tsubsts sub t"
+proof (induction \<Gamma> e t rule: typecheckn.induct)
+  case (tcn_lam \<Gamma> x t\<^sub>1 e t\<^sub>2)
+  hence "map_option (tsubsts sub) \<circ> \<Gamma>(x \<mapsto> t\<^sub>1) \<turnstile>\<^sub>n tsubstt sub e : tsubsts sub t\<^sub>2" by blast
+  hence "map_option (tsubsts sub) \<circ> \<Gamma> \<turnstile>\<^sub>n tsubstt sub (TLam x t\<^sub>1 e) : tsubsts sub (Arrow t\<^sub>1 t\<^sub>2)" 
+    by simp
+  thus ?case by blast
+qed simp_all
+
+lemma [simp]: "typecheck' \<Gamma> vs e = Some (e', t, vs', \<Gamma>') \<Longrightarrow> dom \<Gamma>' = dom \<Gamma>"
+proof (induction e arbitrary: \<Gamma> vs e' t vs' \<Gamma>')
+  case (NLam x e)
+  let ?v = "fresh vs"
+  from NLam obtain ee' tt g\<Gamma>' t' where T: "g\<Gamma>' x = Some t' \<and> e' = HLam x t' ee' \<and> 
+    t = Ctor ''Arrow'' [t', tt] \<and> \<Gamma>' = (g\<Gamma>'(x := \<Gamma> x)) \<and>
+      typecheck' (\<Gamma>(x \<mapsto> Var ?v)) (insert ?v vs) e = Some (ee', tt, vs', g\<Gamma>')" 
+        by (auto simp add: Let_def split: option.splits)
+  with NLam have "dom g\<Gamma>' = dom (\<Gamma>(x \<mapsto> Var ?v))" by blast
+  hence "dom (g\<Gamma>'(x := \<Gamma> x)) = dom \<Gamma>" by auto
+  with T show ?case by blast
+next
+  case (NApp e1 e2)
+  then obtain e\<^sub>1' k t\<^sub>1 t\<^sub>2 vvs' g\<Gamma>' e\<^sub>2' t\<^sub>3 \<Gamma>'' sub where T: "k = ''Arrow'' \<and>
+    typecheck' \<Gamma> vs e1 = Some (e\<^sub>1', Ctor k [t\<^sub>1, t\<^sub>2], vvs', g\<Gamma>') \<and> 
+      typecheck' g\<Gamma>' vvs' e2 = Some (e\<^sub>2', t\<^sub>3, vs', \<Gamma>'') \<and> unify t\<^sub>1 t\<^sub>2 = Some sub \<and> 
+        e' = HApp (hsubst sub e\<^sub>1') (hsubst sub e\<^sub>2') \<and> t = subst sub t\<^sub>2 \<and> 
+          \<Gamma>' = map_option (subst sub) \<circ> \<Gamma>''" 
+    by (auto split: option.splits uexpr.splits list.splits if_splits)
+  with NApp have "dom g\<Gamma>' = dom \<Gamma>" by blast
+  moreover from NApp T have "dom \<Gamma>'' = dom g\<Gamma>'" by blast
+  ultimately have "dom (map_option (subst sub) \<circ> \<Gamma>'') = dom \<Gamma>" by simp
+  with T show ?case by blast
+qed (simp_all split: option.splits)
+
+lemma [simp]: "valid_ty_subst \<Gamma> \<Longrightarrow> typecheck' \<Gamma> vs e = Some (e', t, vs', \<Gamma>') \<Longrightarrow> 
+  valid_ty_subst \<Gamma>' \<and> valid_ty_uexpr t \<and> valid_ty_hexpr e'"
+proof (induction e arbitrary: \<Gamma> vs e' t vs' \<Gamma>')
+  case (NLam x e)
+  let ?v = "fresh vs"
+  from NLam obtain ee' tt g\<Gamma>' t' where T: "g\<Gamma>' x = Some t' \<and> 
+    typecheck' (\<Gamma>(x \<mapsto> Var ?v)) (insert ?v vs) e = Some (ee', tt, vs', g\<Gamma>') \<and> 
+      e' = HLam x t' ee' \<and> t = Ctor ''Arrow'' [t', tt] \<and> \<Gamma>' = (g\<Gamma>'(x := \<Gamma> x))" 
+    by (auto simp add: Let_def split: option.splits prod.splits)
+  from NLam have "valid_ty_subst (\<Gamma>(x \<mapsto> Var ?v))" by simp
+  with NLam T have X: "valid_ty_subst g\<Gamma>' \<and> valid_ty_uexpr tt \<and> valid_ty_hexpr ee'" by blast
+  with T have "valid_ty_uexpr t'" by auto
+  with NLam X have "valid_ty_subst (g\<Gamma>'(x := \<Gamma> x)) \<and> valid_ty_uexpr (Ctor ''Arrow'' [t', tt]) \<and> 
+    valid_ty_hexpr (HLam x t' ee')" by simp
+  with T show ?case by blast
+next
+  case (NApp e1 e2)
+  from NApp(4) obtain e\<^sub>1' t\<^sub>1 t\<^sub>2 vvs' g\<Gamma>' e\<^sub>2' t\<^sub>3 g\<Gamma>'' sub where T: "unify t\<^sub>1 t\<^sub>2 = Some sub \<and> 
+    t = subst sub t\<^sub>2 \<and> e' = HApp (hsubst sub e\<^sub>1') (hsubst sub e\<^sub>2') \<and> 
+      \<Gamma>' = map_option (subst sub) \<circ> g\<Gamma>'' \<and> 
+        typecheck' \<Gamma> vs e1 = Some (e\<^sub>1', Ctor ''Arrow'' [t\<^sub>1, t\<^sub>2], vvs', g\<Gamma>') \<and>
+          typecheck' g\<Gamma>' vvs' e2 = Some (e\<^sub>2', t\<^sub>3, vs', g\<Gamma>'')" 
+    by (auto split: option.splits prod.splits uexpr.splits list.splits if_splits)
+  moreover with NApp have "valid_ty_subst g\<Gamma>' \<and> valid_ty_uexpr (Ctor ''Arrow'' [t\<^sub>1, t\<^sub>2]) \<and> 
+    valid_ty_hexpr e\<^sub>1'" by blast
+  moreover with NApp T have "valid_ty_subst g\<Gamma>'' \<and> valid_ty_uexpr t\<^sub>3 \<and> 
+    valid_ty_hexpr e\<^sub>2'" by blast
+  ultimately have "valid_ty_subst g\<Gamma>'' \<and> valid_ty_subst sub \<and> valid_ty_uexpr t\<^sub>2 \<and> 
+    valid_ty_hexpr e\<^sub>1' \<and> valid_ty_hexpr e\<^sub>2'" by auto
+  hence "valid_ty_subst (map_option (subst sub) \<circ> g\<Gamma>'') \<and> valid_ty_uexpr (subst sub t\<^sub>2) \<and> 
+    valid_ty_hexpr (HApp (hsubst sub e\<^sub>1') (hsubst sub e\<^sub>2'))" by simp
+  with T show ?case by blast
+qed (auto split: option.splits)
+
+lemma [elim]: "valid_ty_subst \<Gamma> \<Longrightarrow> typecheck' \<Gamma> vs e = Some (e', t, vs', \<Gamma>') \<Longrightarrow> valid_ty_uexpr t"
+  by simp
+
+lemma [simp]: "typecheck' \<Gamma> vs e = Some (e', t, vs', \<Gamma>') \<Longrightarrow> valid_ty_subst \<Gamma> \<Longrightarrow> 
+  map_option typeify \<circ> \<Gamma>' \<turnstile>\<^sub>n solidify e' : typeify t"
+proof (induction e arbitrary: \<Gamma> vs e' t vs' \<Gamma>')
+  case (NLam x e)
+  let ?v = "fresh vs"
+  from NLam obtain ee' tt g\<Gamma>' t' where T: "g\<Gamma>' x = Some t' \<and> 
+    typecheck' (\<Gamma>(x \<mapsto> Var ?v)) (insert ?v vs) e = Some (ee', tt, vs', g\<Gamma>') \<and> 
+      e' = HLam x t' ee' \<and> t = Ctor ''Arrow'' [t', tt] \<and> \<Gamma>' = (g\<Gamma>'(x := \<Gamma> x))" 
+    by (auto simp add: Let_def split: option.splits prod.splits)
+  hence X: "g\<Gamma>' = (\<Gamma>'(x \<mapsto> t'))" by auto
+  from NLam have "valid_ty_subst (\<Gamma>(x \<mapsto> Var ?v))" by simp
+  with NLam(1) T have "map_option typeify \<circ> g\<Gamma>' \<turnstile>\<^sub>n solidify ee' : typeify tt" by blast
+  with X have "map_option typeify \<circ> \<Gamma>' \<turnstile>\<^sub>n solidify (HLam x t' ee') : 
+    typeify (Ctor ''Arrow'' [t', tt])" by simp
+  with T show ?case by blast
+next
+  case (NApp e1 e2)
+  from NApp(3) obtain e\<^sub>1' t\<^sub>1 t\<^sub>2 vvs' g\<Gamma>' e\<^sub>2' t\<^sub>3 g\<Gamma>'' sub where T: "unify t\<^sub>1 t\<^sub>2 = Some sub \<and> 
+    t = subst sub t\<^sub>2 \<and> e' = HApp (hsubst sub e\<^sub>1') (hsubst sub e\<^sub>2') \<and> 
+      \<Gamma>' = map_option (subst sub) \<circ> g\<Gamma>'' \<and> 
+        typecheck' \<Gamma> vs e1 = Some (e\<^sub>1', Ctor ''Arrow'' [t\<^sub>1, t\<^sub>2], vvs', g\<Gamma>') \<and>
+          typecheck' g\<Gamma>' vvs' e2 = Some (e\<^sub>2', t\<^sub>3, vs', g\<Gamma>'')" 
+    by (auto split: option.splits prod.splits uexpr.splits list.splits if_splits)
+  with NApp(4) have X: "valid_ty_subst g\<Gamma>' \<and> valid_ty_uexpr (Ctor ''Arrow'' [t\<^sub>1, t\<^sub>2]) \<and> 
+    valid_ty_hexpr e\<^sub>1'" by fastforce
+  with NApp T have Z: "map_option typeify \<circ> g\<Gamma>'' \<turnstile>\<^sub>n solidify e\<^sub>2' : typeify t\<^sub>3" by blast
+  from T X have Y: "valid_ty_subst g\<Gamma>'' \<and> valid_ty_uexpr t\<^sub>3 \<and> valid_ty_hexpr e\<^sub>2'" by fastforce
+
+
+  from NApp T have "map_option typeify \<circ> g\<Gamma>' \<turnstile>\<^sub>n solidify e\<^sub>1' : typeify (Ctor ''Arrow'' [t\<^sub>1, t\<^sub>2])" by blast
+  hence "map_option typeify \<circ> g\<Gamma>' \<turnstile>\<^sub>n solidify e\<^sub>1' : Arrow (typeify t\<^sub>1) (typeify t\<^sub>2)" by simp
+
+
+
+
+  have "map_option typeify \<circ> g\<Gamma>'' \<turnstile>\<^sub>n solidify e\<^sub>1' : Arrow (typeify t\<^sub>3) (typeify t\<^sub>2)" by simp
+  with Z have "map_option typeify \<circ> g\<Gamma>'' \<turnstile>\<^sub>n TApp (solidify e\<^sub>1') (solidify e\<^sub>2') : typeify t\<^sub>2" by simp
+  hence "map_option (tsubsts sub) \<circ> (map_option typeify \<circ> g\<Gamma>'') \<turnstile>\<^sub>n 
+    tsubstt sub (TApp (solidify e\<^sub>1') (solidify e\<^sub>2')) : tsubsts sub (typeify t\<^sub>2)" 
+      by (metis tc_tsubstt)
+  with X Y have "map_option typeify \<circ> (map_option (subst sub) \<circ> g\<Gamma>'') \<turnstile>\<^sub>n 
+    solidify (HApp (hsubst sub e\<^sub>1') (hsubst sub e\<^sub>2')) : typeify (subst sub t\<^sub>2)" by simp
+  with T show ?case by blast
+qed (auto split: option.splits)
 
 lemma [simp]: "typecheck e = Some (e\<^sub>t, t) \<Longrightarrow> Map.empty \<turnstile>\<^sub>n e\<^sub>t : t"
-  by simp
+proof -
+  assume "typecheck e = Some (e\<^sub>t, t)"
+  then obtain e' tt vs \<Gamma> where T: "typecheck' Map.empty {} e = Some (e', tt, vs, \<Gamma>) \<and> 
+    e\<^sub>t = solidify e' \<and> t = typeify tt" by (auto split: option.splits)
+  moreover hence "map_option typeify \<circ> \<Gamma> \<turnstile>\<^sub>n solidify e' : typeify tt" by auto
+  moreover from T have "dom \<Gamma> = dom Map.empty" by force
+  ultimately show "Map.empty \<turnstile>\<^sub>n e\<^sub>t : t" by simp
+qed
+
+lemma erase_solidify [simp]: "valid_ty_subst \<Gamma> \<Longrightarrow> typecheck' \<Gamma> vs e = Some (e', t, vs', \<Gamma>') \<Longrightarrow> 
+  e = erase (solidify e')"
+proof (induction e arbitrary: \<Gamma> vs e' t vs' \<Gamma>')
+  case (NLam x e)
+  let ?v = "fresh vs"
+  from NLam(3) obtain ee' tt g\<Gamma>' t' where T: "g\<Gamma>' x = Some t' \<and> e' = HLam x t' ee' \<and> 
+    t = Ctor ''Arrow'' [t', tt] \<and> \<Gamma>' = g\<Gamma>'(x := \<Gamma> x) \<and> 
+      typecheck' (\<Gamma>(x \<mapsto> Var ?v)) (insert ?v vs) e = Some (ee', tt, vs', g\<Gamma>')" 
+    by (auto simp add: Let_def split: option.splits)
+  from NLam have "valid_ty_subst (\<Gamma>(x \<mapsto> Var ?v))" by simp
+  with NLam(1) T have "e = erase (solidify ee')" by blast
+  with T show ?case by simp
+next
+  case (NApp e1 e2)
+  from NApp(4) obtain e\<^sub>1' t\<^sub>1 t\<^sub>2 vvs' g\<Gamma>' e\<^sub>2' t\<^sub>3 g\<Gamma>'' sub where T: "unify t\<^sub>1 t\<^sub>2 = Some sub \<and> 
+    t = subst sub t\<^sub>2 \<and> e' = HApp (hsubst sub e\<^sub>1') (hsubst sub e\<^sub>2') \<and> 
+      \<Gamma>' = map_option (subst sub) \<circ> g\<Gamma>'' \<and> 
+        typecheck' \<Gamma> vs e1 = Some (e\<^sub>1', Ctor ''Arrow'' [t\<^sub>1, t\<^sub>2], vvs', g\<Gamma>') \<and>
+          typecheck' g\<Gamma>' vvs' e2 = Some (e\<^sub>2', t\<^sub>3, vs', g\<Gamma>'')" 
+    by (auto split: option.splits prod.splits uexpr.splits list.splits if_splits)
+  moreover with NApp(3) have X: "valid_ty_subst g\<Gamma>' \<and> valid_ty_uexpr (Ctor ''Arrow'' [t\<^sub>1, t\<^sub>2]) \<and> 
+    valid_ty_hexpr e\<^sub>1'" by fastforce
+  moreover with T have "valid_ty_subst g\<Gamma>'' \<and> valid_ty_uexpr t\<^sub>3 \<and> valid_ty_hexpr e\<^sub>2'" by fastforce
+  moreover from NApp T have "e1 = erase (solidify e\<^sub>1')" by blast
+  moreover from NApp T X have "e2 = erase (solidify e\<^sub>2')" by blast
+  ultimately show ?case by simp
+qed (auto simp add: Let_def split: option.splits)
 
 lemma [simp]: "typecheck e = Some (e\<^sub>t, t) \<Longrightarrow> e = erase e\<^sub>t"
-  by simp
+proof -
+  assume "typecheck e = Some (e\<^sub>t, t)"
+  then obtain e' tt vs \<Gamma> where T: "typecheck' Map.empty {} e = Some (e', tt, vs, \<Gamma>) \<and> 
+    e\<^sub>t = solidify e' \<and> t = typeify tt" by (auto split: option.splits)
+  moreover have "valid_ty_subst Map.empty" by simp
+  ultimately have "e = erase (solidify e')" by (metis erase_solidify)
+  with T show ?thesis by simp
+qed
+
+lemma [dest]: "NVar x = erase e\<^sub>t \<Longrightarrow> e\<^sub>t = TVar x"
+  by (induction e\<^sub>t) simp_all
+
+lemma [dest]: "NLam x e = erase e\<^sub>t \<Longrightarrow> \<exists>t e\<^sub>t'. e\<^sub>t = TLam x t e\<^sub>t' \<and> e = erase e\<^sub>t'"
+  by (induction e\<^sub>t) simp_all
+
+lemma [simp]: "typecheck' \<Gamma> vs e = None \<Longrightarrow> \<nexists>e\<^sub>t t. (map_option typeify \<circ> \<Gamma> \<turnstile>\<^sub>n e\<^sub>t : t) \<and> e = erase e\<^sub>t"
+proof (induction e arbitrary: \<Gamma> vs)
+  case (NVar x)
+  hence X: "\<Gamma> x = None" by (simp split: option.splits)
+  have "\<And>e\<^sub>t. NVar x = erase e\<^sub>t \<Longrightarrow> \<nexists>t. map_option typeify \<circ> \<Gamma> \<turnstile>\<^sub>n e\<^sub>t : t"
+  proof 
+    fix e\<^sub>t
+    assume "NVar x = erase e\<^sub>t" 
+    hence "e\<^sub>t = TVar x" by blast
+    moreover assume "\<exists>t. map_option typeify \<circ> \<Gamma> \<turnstile>\<^sub>n e\<^sub>t : t"
+    ultimately obtain t where "(map_option typeify \<circ> \<Gamma>) x = Some t" by blast
+    with X show False by simp
+  qed
+  thus ?case by blast
+next
+  case (NLam x e)
+  let ?v = "fresh vs"
+  have "\<And>e\<^sub>t. NLam x e = erase e\<^sub>t \<Longrightarrow> \<nexists>t. map_option typeify \<circ> \<Gamma> \<turnstile>\<^sub>n e\<^sub>t : t"
+  proof
+    fix e\<^sub>t
+    assume "NLam x e = erase e\<^sub>t" 
+    then obtain t\<^sub>1 e\<^sub>t' where E: "e\<^sub>t = TLam x t\<^sub>1 e\<^sub>t' \<and> e = erase e\<^sub>t'" by blast
+    moreover assume "\<exists>t. map_option typeify \<circ> \<Gamma> \<turnstile>\<^sub>n e\<^sub>t : t"
+    ultimately obtain t\<^sub>2 where "(map_option typeify \<circ> \<Gamma>)(x \<mapsto> t\<^sub>1) \<turnstile>\<^sub>n e\<^sub>t' : t\<^sub>2" by blast
+    show False
+    proof (cases "typecheck' (\<Gamma>(x \<mapsto> Var ?v)) (insert ?v vs) e")
+      case None
+      with NLam E have "\<And>t. \<not> map_option typeify \<circ> (\<Gamma>(x \<mapsto> Var ?v)) \<turnstile>\<^sub>n e\<^sub>t' : t" by blast
+    
+    
+      show False by blast
+    next
+      case (Some a)
+      with NLam have "\<exists>e' t vs' \<Gamma>'. typecheck' (\<Gamma>(x \<mapsto> Var ?v)) (insert ?v vs) e = Some (e', t, vs', \<Gamma>') \<and> \<Gamma>' x = None" 
+        by (auto simp add: Let_def split: option.splits prod.splits)
+    
+    
+      show False by blast
+    qed
+  qed
+  thus ?case by blast
+next
+  case (NApp e1 e2)
+  then show ?case by simp
+qed simp_all
 
 lemma typecheck_fails [simp]: "typecheck e = None \<Longrightarrow> \<nexists>e\<^sub>t t. (Map.empty \<turnstile>\<^sub>n e\<^sub>t : t) \<and> e = erase e\<^sub>t"
   by simp
@@ -35,7 +367,59 @@ lemma [simp]: "erase (substt x e' e) = substn x (erase e') (erase e)"
 theorem completeness [simp]: "e \<Down>\<^sub>t v \<Longrightarrow> erase e \<Down> erase v"
   by (induction e v rule: evalt.induct) simp_all
 
-theorem correctness: "e \<Down> v \<Longrightarrow> typecheck e = Some (e\<^sub>t, t) \<Longrightarrow> typecheck v = Some (v\<^sub>t, t) \<Longrightarrow> e\<^sub>t \<Down>\<^sub>t v\<^sub>t"
-  by (induction e v rule: evaln.induct) simp_all
+lemma [simp]: "all_varst (tsubstt sub e) = all_varst e"
+  by (induction e) simp_all
+
+lemma [simp]: "tsubstt sub (subst_vart y x e) = subst_vart y x (tsubstt sub e)"
+  by (induction e) simp_all
+
+lemma [simp]: "tsubstt sub (substt x v e) = substt x (tsubstt sub v) (tsubstt sub e)"
+  by (induction x v e rule: substt.induct) (simp_all add: Let_def)
+
+lemma [simp]: "e \<Down>\<^sub>t v \<Longrightarrow> tsubstt sub e \<Down>\<^sub>t tsubstt sub v"
+  by (induction e v rule: evalt.induct) simp_all
+
+lemma correctness' [simp]: "e \<Down> v \<Longrightarrow> typecheck' \<Gamma> vs e = Some (e\<^sub>t, t1, vs', \<Gamma>') \<Longrightarrow> 
+  typecheck' \<Gamma> vs v = Some (v\<^sub>t, t2, vs'', \<Gamma>'') \<Longrightarrow> valid_ty_subst \<Gamma> \<Longrightarrow> typeify t1 = typeify t2 \<Longrightarrow> 
+    solidify e\<^sub>t \<Down>\<^sub>t solidify v\<^sub>t"
+proof (induction e v arbitrary: \<Gamma> vs e\<^sub>t t1 vs' \<Gamma>' v\<^sub>t t2 vs'' \<Gamma>'' rule: evaln.induct)
+  case (evn_app e\<^sub>1 x e\<^sub>1' e\<^sub>2 v\<^sub>2 v)
+  from evn_app(7) obtain e\<^sub>1'' t\<^sub>1 t\<^sub>2 vs\<^sub>1' \<Gamma>\<^sub>1' e\<^sub>2' t\<^sub>3 \<Gamma>\<^sub>2' sub where T: "t1 = subst sub t\<^sub>2 \<and> 
+    e\<^sub>t = HApp (hsubst sub e\<^sub>1'') (hsubst sub e\<^sub>2') \<and> \<Gamma>' = map_option (subst sub) \<circ> \<Gamma>\<^sub>2' \<and>
+      typecheck' \<Gamma> vs e\<^sub>1 = Some (e\<^sub>1'', Ctor ''Arrow'' [t\<^sub>1, t\<^sub>2], vs\<^sub>1', \<Gamma>\<^sub>1') \<and>
+        typecheck' \<Gamma>\<^sub>1' vs\<^sub>1' e\<^sub>2 = Some (e\<^sub>2', t\<^sub>3, vs', \<Gamma>\<^sub>2') \<and> unify t\<^sub>1 t\<^sub>2 = Some sub" 
+    by (auto split: option.splits if_splits uexpr.splits list.splits)
+  with evn_app(9) have X: "valid_ty_subst \<Gamma>\<^sub>1' \<and> valid_ty_uexpr (Ctor ''Arrow'' [t\<^sub>1, t\<^sub>2]) \<and> 
+    valid_ty_hexpr e\<^sub>1''" by fastforce
+  with T have Y: "valid_ty_subst \<Gamma>\<^sub>2' \<and> valid_ty_uexpr t\<^sub>3 \<and> valid_ty_hexpr e\<^sub>2'" by fastforce
+
+
+  from evn_app T have "typecheck' \<Gamma> vs (NLam x e\<^sub>1') = Some (xv\<^sub>t, xt2, xvs'', x\<Gamma>'') \<Longrightarrow> 
+    Arrow (typeify t\<^sub>1) (typeify t\<^sub>2) = typeify xt2 \<Longrightarrow> solidify e\<^sub>1'' \<Down>\<^sub>t solidify xv\<^sub>t" by auto
+
+  from evn_app T have "typecheck' \<Gamma>\<^sub>1' vs\<^sub>1' v\<^sub>2 = Some (xv\<^sub>t, xt2, xvs'', x\<Gamma>'') \<Longrightarrow> 
+    typeify t\<^sub>3 = typeify xt2 \<Longrightarrow> valid_ty_subst \<Gamma>\<^sub>1' \<Longrightarrow> solidify e\<^sub>2' \<Down>\<^sub>t solidify xv\<^sub>t" by blast
+
+  from evn_app have "e\<^sub>1 \<Down> NLam x e\<^sub>1'" by simp
+  from evn_app have "e\<^sub>2 \<Down> v\<^sub>2" by simp
+  from evn_app have "substn x v\<^sub>2 e\<^sub>1' \<Down> v" by simp
+
+
+
+
+  from evn_app have "typecheck' x\<Gamma> xvs (substn x v\<^sub>2 e\<^sub>1') = Some (xe\<^sub>t, xt1, xvs', x\<Gamma>') \<Longrightarrow>
+    typecheck' x\<Gamma> xvs v = Some (xv\<^sub>t, xt2, xvs'', x\<Gamma>'') \<Longrightarrow> valid_ty_subst x\<Gamma> \<Longrightarrow> typeify xt1 = typeify xt2 \<Longrightarrow> 
+      solidify xe\<^sub>t \<Down>\<^sub>t solidify xv\<^sub>t" by simp
+  from evn_app have "typecheck' \<Gamma> vs v = Some (v\<^sub>t, t2, vs'', \<Gamma>'')" by simp
+  from evn_app have "typeify t1 = typeify t2" by simp
+
+
+  have "tsubstt sub (TApp (solidify e\<^sub>1'') (solidify e\<^sub>2')) \<Down>\<^sub>t solidify v\<^sub>t" by simp
+  with T X Y show ?case by simp
+qed (auto simp add: Let_def split: option.splits)
+
+theorem correctness: "e \<Down> v \<Longrightarrow> typecheck e = Some (e\<^sub>t, t) \<Longrightarrow> typecheck v = Some (v\<^sub>t, t) \<Longrightarrow> 
+    e\<^sub>t \<Down>\<^sub>t v\<^sub>t"
+  by (auto split: option.splits)
 
 end
