02Typed/Type.thy
@@ -3,12 +3,12 @@ theory Type
 begin
 
 datatype ty = 
-  TVar var
+  TyVar var
   | Base 
   | Arrow ty ty
 
 primrec tsubst_var :: "var \<Rightarrow> var \<Rightarrow> ty \<Rightarrow> ty" where
-  "tsubst_var x x' (TVar y) = TVar (if x = y then x' else y)"
+  "tsubst_var x x' (TyVar y) = TyVar (if x = y then x' else y)"
 | "tsubst_var x x' Base = Base"
 | "tsubst_var x x' (Arrow t\<^sub>1 t\<^sub>2) = Arrow (tsubst_var x x' t\<^sub>1) (tsubst_var x x' t\<^sub>2)"
 
@@ -16,7 +16,7 @@ lemma [simp]: "size (tsubst_var x x' t) = size t"
   by (induction t) simp_all
 
 fun tsubst :: "var \<Rightarrow> ty \<Rightarrow> ty \<Rightarrow> ty" where
-  "tsubst x t' (TVar y) = (if x = y then t' else TVar y)"
+  "tsubst x t' (TyVar y) = (if x = y then t' else TyVar y)"
 | "tsubst x t' Base = Base"
 | "tsubst x t' (Arrow t\<^sub>1 t\<^sub>2) = Arrow (tsubst x t' t\<^sub>1) (tsubst x t' t\<^sub>2)"
 
